intermediate/Veritas.Intermediate.Thread.fsti
@@ -75,27 +75,30 @@ let blum_add_elem #vcfg (e:logS_entry vcfg {is_blum_add e}):
   match e with
   | AddB_S s r t j -> MHDom r t j
 
-val blum_add_seq (#vcfg:_) (tl: verifiable_log vcfg): S.seq ms_hashfn_dom
+val blum_add_seq (#vcfg:_) (ep: epoch) (tl: verifiable_log vcfg): S.seq ms_hashfn_dom
 
 val add_seq_map (#vcfg:_) (tl: verifiable_log vcfg) (i: seq_index tl{is_blum_add (index tl i)}):
-  (j: SA.seq_index (blum_add_seq tl){S.index (blum_add_seq tl) j =
-                                     blum_add_elem (index tl i)})
+  (let be = blum_add_elem (index tl i) in
+   let ep = epoch_of be in
+   let add_seq = blum_add_seq ep tl in
 
-val add_seq_inv_map (#vcfg:_) (tl: verifiable_log vcfg) (j: SA.seq_index (blum_add_seq tl)):
+   j: SA.seq_index add_seq {S.index add_seq j = be})
+
+val add_seq_inv_map (#vcfg:_) (ep: epoch) (tl: verifiable_log vcfg) (j: SA.seq_index (blum_add_seq ep tl)):
   (i: seq_index tl {is_blum_add (index tl i) /\
-              blum_add_elem (index tl i) = S.index (blum_add_seq tl) j /\
-              add_seq_map tl i = j})
+                    blum_add_elem (index tl i) = S.index (blum_add_seq ep tl) j /\
+                    epoch_of (blum_add_elem (index tl i)) = ep /\
+                    add_seq_map tl i = j})
 
 val lemma_add_seq_inv (#vcfg:_) (tl: verifiable_log vcfg) (i: seq_index tl{is_blum_add (index tl i)}):
-  Lemma (ensures (add_seq_inv_map tl (add_seq_map tl i) = i))
+  Lemma (ensures (let be = blum_add_elem (index tl i) in
+                  let ep = epoch_of be in
+                  add_seq_inv_map ep tl (add_seq_map tl i) = i))
         [SMTPat (add_seq_map tl i)]
 
 (* aggregated hash upto current epoch *)
-let hadd #vcfg (tl: verifiable_log vcfg): ms_hash_value =
-  let vs = verify tl in
-  match vs with
-  | Valid _ _ (MkTimestamp ep _) ha _ ->
-    IntV.aggr_epoch_hashes_upto ha ep
+let hadd #vcfg (tl: verifiable_log vcfg) (ep: epoch): ms_hash_value =
+  Valid?.hadd (verify tl) ep
 
 (* the verifier state after processing i entries *)
 let state_at #vcfg (tl: verifiable_log vcfg) (i:nat{i <= length tl}): st:vtls _{Valid? st} =
@@ -107,9 +110,8 @@ val lemma_state_transition (#vcfg:_)
   Lemma (state_at tl (i + 1) ==
          verify_step (state_at tl i) (index tl i))
 
-val lemma_hadd_correct (#vcfg:_) (tl: verifiable_log vcfg):
-  Lemma (ensures (hadd tl = ms_hashfn (blum_add_seq tl)))
-        [SMTPat (verifiable tl)]
+val lemma_hadd_correct (#vcfg:_) (ep: epoch) (tl: verifiable_log vcfg):
+  Lemma (ensures (hadd tl ep = ms_hashfn (blum_add_seq ep tl)))
 
 let blum_evict_elem (#vcfg:_) (tl: verifiable_log vcfg) (i:seq_index tl{is_evict_to_blum (index tl i)}): ms_hashfn_dom =
   let (tid, _) = tl in
@@ -119,28 +121,31 @@ let blum_evict_elem (#vcfg:_) (tl: verifiable_log vcfg) (i:seq_index tl{is_evict
   let vs = verify tli in
   IntV.blum_evict_elem vs e tid
 
-val blum_evict_seq (#vcfg:_) (tl: verifiable_log vcfg): S.seq ms_hashfn_dom
+val blum_evict_seq (#vcfg:_) (ep: epoch) (tl: verifiable_log vcfg): S.seq ms_hashfn_dom
 
-let hevict #vcfg (tl: verifiable_log vcfg): ms_hash_value =
-  let vs = verify tl in
-  match vs with
-  | Valid _ _ (MkTimestamp ep _) _ he ->
-    IntV.aggr_epoch_hashes_upto he ep
+let hevict #vcfg (tl: verifiable_log vcfg) (ep: epoch): ms_hash_value =
+  Valid?.hevict (verify tl) ep
 
-val lemma_hevict_correct (#vcfg:_) (tl: verifiable_log vcfg):
-  Lemma (hevict tl = ms_hashfn (blum_evict_seq tl))
+val lemma_hevict_correct (#vcfg:_) (ep: epoch) (tl: verifiable_log vcfg):
+  Lemma (hevict tl ep = ms_hashfn (blum_evict_seq ep tl))
 
 val evict_seq_map (#vcfg:_) (tl: verifiable_log vcfg) (i: seq_index tl{is_evict_to_blum (index tl i)}):
-  (j: SA.seq_index (blum_evict_seq tl) {S.index (blum_evict_seq tl) j =
-                                        blum_evict_elem tl i})
+  (let be = blum_evict_elem tl i in
+   let ep = epoch_of be in
+   let evict_seq = blum_evict_seq ep tl in
 
-val evict_seq_inv_map (#vcfg:_) (tl: verifiable_log vcfg) (j: SA.seq_index (blum_evict_seq tl)):
+   j: SA.seq_index (blum_evict_seq ep tl) {S.index evict_seq j = be})
+
+val evict_seq_inv_map (#vcfg:_) (ep: epoch) (tl: verifiable_log vcfg) (j: SA.seq_index (blum_evict_seq ep tl)):
   (i: seq_index tl{is_evict_to_blum (index tl i) /\
-             blum_evict_elem tl i = S.index (blum_evict_seq tl) j /\
-             evict_seq_map tl i = j})
+                   blum_evict_elem tl i = S.index (blum_evict_seq ep tl) j /\
+                   epoch_of (blum_evict_elem tl i) = ep /\
+                   evict_seq_map tl i = j})
 
 val lemma_evict_seq_inv (#vcfg:_) (tl: verifiable_log vcfg) (i: seq_index tl{is_evict_to_blum (index tl i)}):
-  Lemma (ensures (evict_seq_inv_map tl (evict_seq_map tl i) = i))
+  Lemma (ensures (let be = blum_evict_elem tl i in
+                  let ep = epoch_of be in
+                  evict_seq_inv_map ep tl (evict_seq_map tl i) = i))
         [SMTPat (evict_seq_map tl i)]
 
 val lemma_blum_evict_elem_prefix (#vcfg:_) (tl: verifiable_log vcfg) (i: nat{i <= length tl})
@@ -153,11 +158,14 @@ val lemma_add_clock (#vcfg:_) (tl: verifiable_log vcfg) (i: seq_index tl{is_blum
 val lemma_evict_clock (#vcfg:_) (tl: verifiable_log vcfg) (i: seq_index tl{is_evict_to_blum (index tl i)}):
   Lemma (timestamp_of (blum_evict_elem tl i) = clock tl i)
 
-val lemma_evict_elem_tid (#vcfg:_) (tl:verifiable_log vcfg):
-  Lemma (all (is_of_thread_id (thread_id_of tl)) (blum_evict_seq tl))
+val lemma_evict_elem_tid (#vcfg:_) (ep: epoch) (tl:verifiable_log vcfg):
+  Lemma (all (is_of_thread_id (thread_id_of tl)) (blum_evict_seq ep tl))
 
 val lemma_clock_monotonic (#vcfg:_) (tl: verifiable_log vcfg) (i:seq_index tl) (j:seq_index tl{j >= i}):
   Lemma (clock tl i `ts_leq` clock tl j)
 
-val lemma_evict_elem_unique (#vcfg:_) (tl: verifiable_log vcfg) (i1 i2: SA.seq_index (blum_evict_seq tl)):
-  Lemma (i1 <> i2 ==> S.index (blum_evict_seq tl) i1 <> S.index (blum_evict_seq tl) i2)
+val lemma_evict_elem_unique (#vcfg:_)
+  (ep: epoch)
+  (tl: verifiable_log vcfg)
+  (i1 i2: SA.seq_index (blum_evict_seq ep tl)):
+  Lemma (i1 <> i2 ==> S.index (blum_evict_seq ep tl) i1 <> S.index (blum_evict_seq ep tl) i2)
